src/ReactorModel/Execution/Theorems/Grouped/Steps.lean
@@ -6,18 +6,17 @@ open ReactorType
 
 namespace Execution.Grouped
 
-variable [Indexable α]
-
-inductive Step (s₁ s₂ : State α)
+inductive Step [Indexable α] (s₁ s₂ : State α)
   | inst : (s₁ ↓ᵢ| s₂) → Step s₁ s₂
   | time : (s₁ ↓ₜ s₂) → Step s₁ s₂
 
 namespace Step
 
-variable {s₁ s₂ : State α}
+variable [Indexable α] {s₁ s₂ : State α}
 
-theorem deterministic (e₁ : Step s s₁) (e₂ : Step s s₂) : s₁ = s₂ := by
-  sorry
+theorem tag_le : (Step s₁ s₂) → s₁.tag ≤ s₂.tag
+  | inst e => e.preserves_tag ▸ le_refl _
+  | time e => le_of_lt e.tag_lt
 
 instance : Coe (s₁ ↓ᵢ| s₂) (Step s₁ s₂) where
   coe := inst
@@ -27,17 +26,25 @@ instance : Coe (s₁ ↓ₜ s₂) (Step s₁ s₂) where
 
 end Step
 
-inductive Steps : State α → State α → Type 
+theorem Step.deterministic [Proper α] {s s₁ s₂ : State α} : (Step s s₁) → (Step s s₂) → s₁ = s₂
+  | inst e₁, inst e₂                    => e₁.deterministic e₂
+  | time e₁, time e₂                    => e₁.deterministic e₂
+  | inst e₁, time e₂ | time e₂, inst e₁ => e₁.not_closed e₂.closed |>.elim
+
+inductive Steps [Indexable α] : State α → State α → Type 
   | refl : Steps s s
   | step : (Step s₁ s₂) → (Steps s₂ s₃) → Steps s₁ s₃ 
 
 namespace Steps
 
-theorem tag_lt {s₁ : State α} (e : Steps s₁ s₂) : s₁.tag < s₂.tag := by
-  sorry
+theorem tag_le [Indexable α] {s₁ s₂ : State α} (e : Steps s₁ s₂) : s₁.tag ≤ s₂.tag := by
+  induction e
+  case refl => rfl
+  case step e _ hi => exact le_trans e.tag_le hi
 
-theorem deterministic {s₁ s₂ : State α} (e₁ : Steps s s₁) (e₂ : Steps s s₂) (n : s.Nontrivial)
-    (ht : s₁.tag = s₂.tag) (hp : s₁.progress = s₂.progress) : s₁ = s₂ := by
+theorem deterministic [Proper α] {s s₁ s₂ : State α} 
+    (e₁ : Steps s s₁) (e₂ : Steps s s₂) (n : s.Nontrivial) (ht : s₁.tag = s₂.tag) 
+    (hp : s₁.progress = s₂.progress) : s₁ = s₂ := by
   induction e₁ <;> cases e₂
   case refl.refl => rfl
   case step.step e₁ _ hi _ e₂ e₂' => 
