src/ReactorModel/Execution/Theorems/Execution.lean
@@ -10,7 +10,7 @@ variable [Proper α] {s : State α}
 theorem deterministic 
     (e₁ : s ⇓ s₁) (e₂ : s ⇓ s₂) (ht : s₁.tag = s₂.tag) (hp : s₁.progress = s₂.progress) : s₁ = s₂ := 
   if h : s.Nontrivial 
-  then (e₁.grouped h).deterministic ht hp (e₂.grouped h)
+  then (e₁.grouped h).deterministic h ht hp (e₂.grouped h)
   else e₁.trivial_deterministic h e₂ ht
   
 end Execution
